implement uwp

KLR/Semantics/ProofRules.lean
@@ -10,79 +10,60 @@ import KLR.Semantics.Logic
 import KLR.Semantics.SmallStep
 
 section weakestpre
-open Iris.BI.BIBase KLR.Core Iris NML
+open Iris Iris.BI Iris.BI.BIBase KLR.Core Iris NML SmallStep
 
 variable {DataT : Type _}
 
-/-- Value-value rule: base case for the proof -/
-theorem wpValVal {p1 p2 : ExecState DataT } {v1 v2 : NML.Value DataT} {Φ : NML.Value DataT → NML.Value DataT → PROP DataT} {K}
-    (H1 : toVal p1 = some v1) (H2 : toVal p2 = some v2) :
+/-- Two values are related when they are related by Φ. -/
+theorem wpValVal (H1 : toVal p1 = some v1) (H2 : toVal p2 = some v2) :
     Φ v1 v2 ⊢ wp K p1 p2 Φ := by
-  -- Unfold the WP
-  refine Entails.trans ?_ (Q := ?_) ?G1
-  case G1 =>
-    apply (Iris.BI.equiv_iff.mp ?G2).mp
-    case G2=> exact (@wp_unfold DataT K p1 p2 Φ).symm
-    -- Weird unification bug?
-
-  -- Enter the left case
-  istart; iintro H; ileft; istop
-
-  -- Eliminate the update
-  refine Entails.trans BIUpdate.intro (Q := iprop(|==> Φ v1 v2)) (BIUpdate.mono ?_)
-
-  -- Specialize the exists and conclude
-  istart
-  iintro H
+  -- Unfold the wp
+  refine .trans ?_ (equiv_iff.mp <| wp_unfold.symm).mp
+  -- Enter the left case because the programs are values
+  refine .trans ?_ or_intro_l
+  -- Eliminate the update (the ghost state does not need to be updated)
+  refine .trans ?_ BIUpdate.intro
+  -- Conclude, using the current state
+  iintro HΦ
   iexists v1
   iexists v2
-  isplit r; ipure_intro; exact H1
-  isplit r; ipure_intro; exact H2
-  iexact H
+  isplit r
+  · -- Side condition
+    ipure_intro; exact H1
+  isplit r
+  · -- Side condition
+    ipure_intro; exact H2
+  iexact HΦ
 
-theorem wpPureSync {p1 p2 p1' p2' : ExecState DataT} {Φ : NML.Value DataT → NML.Value DataT → @PROP DataT} {K : LeibnizO Nat}
-    (H1 : SmallStep.PureStep p1 p1')
-    (H2 : SmallStep.PureStep p2 p2')
-    (Hk : 1 ≤ K.car) :
+-- NB. Keeping this code in the repo as an example for writing basic proof rules.
+@[deprecated "Use dwpDesync/dwpResync instead. " (since:="2025/07/31") ]
+theorem wpPureSync {Φ : Value DataT → Value DataT → @PROP DataT}
+    (H1 : PureStep p1 p1') (H2 : PureStep p2 p2') (Hk : 1 ≤ K.car) :
     wp K p1' p2' Φ ⊢ wp K p1 p2 Φ := by
   -- Unfold the WP
-  refine Entails.trans ?_ (Q := ?_) ?G1
-  case G1 =>
-    apply (Iris.BI.equiv_iff.mp ?G2).mp
-    case G2=> exact (@wp_unfold DataT K p1 p2 Φ).symm
-    -- Weird unification bug?
-
-  -- Enter the right case, get state resources, set step numbers
-  istart
-  iintro H
-  iright
-  iintro sl sr Hs
-  istop
+  refine .trans ?_ (equiv_iff.mp <| wp_unfold.symm).mp
+  -- Enter the right case because the programs can step
+  refine .trans ?_ or_intro_r
+  -- Obtain state and wp resources
+  iintro Hwp σₗ σᵣ Hσ
+  -- Eliminate the update (the ghost state does not need to be updated)
   apply Entails.trans _ BIUpdate.intro
-  istart
+  -- We will re-establish the wp for the states after one step of the left
+  -- and right states, ending in (p1', σₗ) and (p2', σᵣ) respectively.
   iintro ⟨Hwp, Hs⟩
-  iexists (p1', sl)
-  iexists (p2', sr)
+  iexists (p1', σₗ)
+  iexists (p2', σᵣ)
   iexists 1
   iexists 1
   isplit r
-  · ipure_intro
-    refine ⟨Nat.one_pos, Nat.one_pos, Hk, Hk, ?_, ?_⟩
-    · exact (NMLSemantics DataT).stepN_1_iff_step.mpr (H1 _)
-    · exact (NMLSemantics DataT).stepN_1_iff_step.mpr (H2 _)
-  istop
-
+  · -- Side condition
+    ipure_intro
+    simp [Hk]
+    refine ⟨stepN_1_iff_step.mpr <| H1 _, stepN_1_iff_step.mpr <| H2 _⟩
   -- Eliminate the later
   refine Entails.trans ?_ Iris.BI.later_intro
-
-  -- Close using the remaining resources
-  istart
-  iintro ⟨Hwp, Hstate⟩
-  isplit l [Hstate]
-  · iexact Hstate
-  · iexact Hwp
-
-
+  -- Conclude
+  exact sep_symm
 
 -- TODO: Port updates for heaps
 theorem update_lemma (σₗ σᵣ : NML.State DataT) :
@@ -91,6 +72,9 @@ theorem update_lemma (σₗ σᵣ : NML.State DataT) :
     state_interp ⟨(ChipMemory.freshSBUFStore σₗ.1).2⟩ ⟨(ChipMemory.freshSBUFStore σᵣ.1).2⟩) :=
   sorry
 
+-- NB. Keeping this code in the repo as an example for writing basic proof rules.
+open ChipMemory in
+@[deprecated "Use dwpDesync/dwpResync instead. " (since:="2025/07/31") ]
 theorem wpAllocSync  {Φ : NML.Value DataT → NML.Value DataT → @PROP DataT} {K : LeibnizO Nat}
     (Hk : 1 ≤ K.car) :
      (∀ ℓₗ ℓᵣ, (ℓₗ [S]⇉ₗ∅) -∗ (ℓᵣ [S]⇉ᵣ∅) -∗ wp K (.run <| p1) (.run <| p2) Φ) ⊢
@@ -98,67 +82,392 @@ theorem wpAllocSync  {Φ : NML.Value DataT → NML.Value DataT → @PROP DataT} 
        (.run <| ⟨.assign none (.alloc Memory.sbuf), locₗ⟩ :: p1)
        (.run <| ⟨.assign none (.alloc Memory.sbuf), loc₂⟩ :: p2)
        Φ := by
-  refine Entails.trans ?_ (Q := ?_) ?G1
-  case G1 =>
-    apply (Iris.BI.equiv_iff.mp ?G2).mp
-    case G2=> exact (@wp_unfold DataT K _ _ Φ).symm
-  iintro ⟨Hrec⟩
-  iright
-  iintro σₗ σᵣ
-  iintro Hσ
-
-  -- Apply update_lemma and eliminate the bupd
-  istop
-  have X := update_lemma σₗ σᵣ
-  have Y := @BI.sep_mono_r (PROP := @PROP DataT) _ _ _ (P := iprop(∀ ℓₗ ℓᵣ, ℓₗ [S]⇉ₗ∅ -∗ ℓᵣ [S]⇉ᵣ∅ -∗ wp K (ExecState.run p1) (ExecState.run p2) Φ)) X
-  apply Entails.trans Y
-  clear X Y
-  apply Entails.trans bupd_frame_l
-  refine BIUpdate.mono ?_
-  istart
-
-
-  iintro ⟨Hrec⟩
-  iexists (.run p1, ⟨ChipMemory.freshSBUFStore σₗ.memory |>.2⟩)
-  iexists (.run p2, ⟨ChipMemory.freshSBUFStore σᵣ.memory |>.2⟩)
+  -- Unfold the wp
+  refine .trans ?_ (equiv_iff.mp <| wp_unfold.symm).mp
+  -- Enter the right case because the programs can step
+  refine .trans ?_ or_intro_r
+  -- Obtain state and wp resources
+  iintro ⟨Hrec⟩ σₗ σᵣ Hσ
+  -- We must update the state to perform the allocation.
+  -- Concretely, will use `update-lemma` (FIXME: rename) to do this.
+  -- `update_lemma` returns resources underneath a basic update modality |==>.
+  -- Because our goal also begins with a basic update modality, we are able to eliminate
+  -- this modality from our updated resource using `BIUpdate.mono`.
+  refine .trans (sep_mono_r <| update_lemma σₗ σᵣ) ?_
+  refine .trans bupd_frame_l (BIUpdate.mono ?_)
+  iintro Hrec
+  -- We will re-establish the wp for the states after the one allocation step of the left
+  -- and right states.
+  iexists (.run p1, ⟨freshSBUFStore σₗ.1 |>.2⟩)
+  iexists (.run p2, ⟨freshSBUFStore σᵣ.1 |>.2⟩)
   iexists 1
   iexists 1
   isplit r
-  · ipure_intro
+  · -- Side condition
+    ipure_intro
     simp [Hk]
     refine ⟨?_, ?_⟩
-    · apply (NMLSemantics DataT).stepN_1_iff_step.mpr
-      apply step.seq (v := Value.uptr <| ChipMemory.freshSBUFStore σₗ.memory |>.1)
-      apply ExprStep.sbuf_alloc rfl
-    · apply (NMLSemantics DataT).stepN_1_iff_step.mpr
-      apply step.seq (v := Value.uptr <| ChipMemory.freshSBUFStore σᵣ.memory |>.1)
-      apply ExprStep.sbuf_alloc rfl
-  istop
-  refine Entails.trans ?_ Iris.BI.later_intro
-  istart
+    · exact stepN_1_iff_step.mpr (.seq <| .sbuf_alloc rfl)
+    · exact stepN_1_iff_step.mpr (.seq <| .sbuf_alloc rfl)
+  -- Eliminate the later
+  refine .trans ?_ Iris.BI.later_intro
+  -- Conclude using the updated resources and Hwp
   iintro ⟨Hwp, ℓₗ, ℓᵣ, Hℓₗ, Hℓᵣ, Hσ⟩
-  simp only []
   ispecialize Hwp ℓₗ ℓᵣ Hℓₗ Hℓᵣ
-  isplit l [Hσ]
+  exact entails_preorder.refl
+
+/-! Desynchronized WP's (dwp)
+
+Many interesting relational proofs will take different steps on the left- and right-handed sides.
+The `dwp` modality allows the left and right programs to take steps independently.
+`dwp` is parameterized by four integers `Lm Rm Lx Rx`. A `dwp Lm Rm Lx Rx` allows the left program
+to take between `Lm` and `Lx` steps (inclusive), likewise with the right program.
+
+The theorem `wpDesync` introduces a `dwp` modality around a `wp k`, where the left and right
+programs must take between 1 and `k` steps each (note: both programs must take at least one step).
+The theorem `wpResync` eliminates a `dwp` modality, provided the minimum number of steps have been
+taken on both sides.
+The `dwp` modality includes a basic update, allowing for each independent step to update the state. -/
+
+/-- The desynchronized weakest precondition modality (dwp). -/
+def dwp (Lm Rm Lx Rx : Nat) (p1 p2 : ExecState DataT) (Φ : ExecState DataT → ExecState DataT → @PROP DataT) :
+    @PROP DataT := iprop(
+  ∀ s1, ∀ s2, state_interp s1 s2 -∗ |==>
+  ∃ p1' p2', Φ p1' p2' ∗ ∃ s1' s2',
+    (∃ nl nr, ⌜Lm ≤ nl ∧ Rm ≤ nr ∧ nl ≤ Lx ∧ nr ≤ Rx ∧
+      SmallStep.StepN nl (p1, s1) (p1', s1') ∧ SmallStep.StepN nr (p2, s2) (p2', s2')⌝ ) ∗
+    state_interp s1' s2')
+
+/-- Introduce a `dwp` around a weakest precondition. -/
+theorem wpDesync : ⊢ dwp 1 1 K.1 K.1 p1 p2 (wp K · · Φf) -∗ wp K p1 p2 Φf := by
+  -- Unfold the wp and dwp
+  refine .trans ?_ <| wand_mono entails_preorder.refl (equiv_iff.mp wp_unfold.symm).mp
+  unfold dwp
+  -- Enter the right case because the programs can step
+  iintro Hdwp
+  iright
+  iintro sl sr Hσ
+  -- Eliminate the bupd modality, gaining access to the updated resources
+  ispecialize Hdwp sl sr Hσ
+  refine .trans Iris.BI.emp_sep.mp (BIUpdate.mono ?_)
+  iintro Hdwp
+  icases Hdwp with ⟨p1', p2', Hwp, s1', s2', ⟨n1, n2, %Hstep⟩, Hupd⟩
+  -- Establish wp in the updated state
+  iexists (p1', s1')
+  iexists (p2', s2')
+  iexists n1
+  iexists n2
+  isplit r
+  · -- Side condition
+    ipure_intro
+    obtain ⟨_, _, _, _, _, _⟩ := Hstep
+    refine ⟨?_, ?_, ?_, ?_, by trivial⟩ <;> try omega
+  -- Eliminate the later
+  refine .trans ?_ later_intro
+  -- Conclude using current resources
+  exact sep_symm
+
+/-- Eliminate a `dwp` that has met its minimum step count. -/
+theorem wpResync : ⊢ Φ p1 p2 -∗ dwp 0 0 Lx Rx p1 p2 Φ := by
+  unfold dwp
+  iintro HΦ s1 s2 Hσ
+  refine .trans ?_ BIUpdate.intro
+  iintro ⟨HΦ, Hσ⟩
+  iexists p1
+  iexists p2
+  isplit l [HΦ]
+  · iexact HΦ
+  iexists s1
+  iexists s2
+  isplit r
+  · iexists 0
+    iexists 0
+    ipure_intro
+    simp only [Nat.le_refl, Nat.zero_le, true_and]
+    refine ⟨StepN.done rfl, StepN.done rfl⟩
   · iexact Hσ
-  · iexact Hwp
 
-/-- Unary weakest precondition
+-- NB. Keeping this code in the repo as an example for writing basic proof rules.
+/-- `dwp` for a single pure step on the left. -/
+@[deprecated "Use dwpL with a PureStep uwp instead. " (since:="2025/07/31") ]
+theorem dwpPureL (Hstep : PureStep p1 p1') (Hx : 0 < Lx := by omega) :
+    ⊢ dwp (Lm - 1) Rm (Lx - 1) Rx p1' p2 Φ -∗ dwp Lm Rm Lx Rx p1 p2 Φ := by
+  -- Unfold the dwp
+  unfold dwp
+  iintro Hdwp sl sr Hσ
+  ispecialize Hdwp sl sr Hσ
+  -- Eliminate the update guarding the dwp
+  refine .trans emp_sep.mp (BIUpdate.mono ?_)
+  iintro Hdwp
+  -- Obtain new resources from the dwp hypothesis
+  icases Hdwp with ⟨p1', p2', HΦ, s1', s2', ⟨nl, nr, %Hstep⟩, Hstate⟩
+  -- Reestablish dwp
+  iexists p1'
+  iexists p2'
+  isplit l [HΦ]
+  · iexact HΦ
+  iexists s1'
+  iexists s2'
+  isplit r
+  · iexists (nl + 1)
+    iexists nr
+    ipure_intro
+    obtain ⟨_, _, _, _, _, _⟩ := Hstep
+    refine ⟨?_, ?_, ?_, ?_, ?_, ?_⟩ <;> try omega
+    refine StepN.step (Hstep sl) ?_
+    trivial
+  · iexact Hstate
 
--/
-structure UWP (DataT : Type _) where
+
+-- NB. Keeping this code in the repo as an example for writing basic proof rules.
+/-- `dwp` for a single pure step on the right. -/
+@[deprecated "Use dwpL with a PureStep uwp instead. " (since:="2025/07/31") ]
+theorem dwpPureR (Hstep : SmallStep.PureStep p2 p2') (Hx : 0 < Rx := by omega) :
+    ⊢ dwp Lm (Rm - 1) Lx (Rx - 1) p1 p2' Φ -∗ dwp Lm Rm Lx Rx p1 p2 Φ := by
+  -- Unfold the dwp
+  unfold dwp
+  iintro Hdwp sl sr Hσ
+  ispecialize Hdwp sl sr Hσ
+  -- Eliminate the update guarding the dwp
+  refine .trans emp_sep.mp (BIUpdate.mono ?_)
+  iintro Hdwp
+  -- Obtain new resources from the dwp hypothesis
+  icases Hdwp with ⟨p1', p2', HΦ, s1', s2', ⟨nl, nr, %Hstep⟩, H⟩
+  -- Reestablish dwp
+  iexists p1'
+  iexists p2'
+  isplit l [HΦ]
+  · iexact HΦ
+  iexists s1'
+  iexists s2'
+  isplit r [H]
+  · iexists nl
+    iexists (nr + 1)
+    ipure_intro
+    obtain ⟨_, _, _, _, _, _⟩ := Hstep
+    refine ⟨?_, ?_, ?_, ?_, ?_, ?_⟩ <;> try omega
+    refine StepN.step (Hstep sr) ?_
+    trivial
+  · iexact H
+
+theorem update_lemma_left (σₗ σᵣ : NML.State DataT)
+      (HL : ChipMemory.get_store σₗ.memory (.sbufUnboundedIndex ℓ₁) = none):
+  state_interp σₗ σᵣ ⊢ |==> ((ChipMemory.freshSBUFStore σₗ.1).1 ⇉ₗ∅ ∗ state_interp ⟨(ChipMemory.freshSBUFStore σₗ.1).2⟩ σᵣ) :=
+  sorry
+
+-- NB. Keeping this code in the repo as an example for writing basic proof rules.
+open ChipIndex in
+/-- `dwp` for a single allocation step on the left. This is a little bit simpler
+than the `uwp` version since it quantifies over the generated location. -/
+theorem dwpAllocL (Hx : 0 < Lx := by omega) :
+    ⊢ (∀ ℓₗ, (ℓₗ [S]⇉ₗ∅) -∗
+        dwp (Lm - 1) Rm (Lx - 1) Rx (.run <| p1'.map (.bind DataT · x (.uptr <| sbufUnboundedIndex ℓₗ))) p2 Φ) -∗
+      dwp Lm Rm Lx Rx (.run <| ⟨.assign (.some x) (.alloc Memory.sbuf), locₗ⟩ :: p1') p2 Φ := by
+  -- Unfold the dwp in the conclusion
+  iintro Hdwp
+  conv => rhs; unfold dwp
+  iintro sl sr Hs
+  -- Update the resources
+  refine .trans (sep_mono_r (update_lemma_left sl sr (ℓ₁ := sl.memory.sbufUnbounded.next_fresh) ?G)) ?_
+  case G =>
+    simp [ChipMemory.get_store]
+    rw [← AllocHeap.get_fresh (t := sl.memory.sbufUnbounded) (H := sl.memory.sbuf_wf)]
+    rfl
+  iintro ⟨Hdwp, Hupd⟩
+  -- Eliminate bupds from the hypotheses but not the conclusion, by duplicating the bupd in the conclusion.
+  istop
+  refine .trans ?_ bupd_idem.mp
+  refine .trans bupd_frame_l (BIUpdate.mono ?_)
+  iintro ⟨Hdwp, ⟨Hfrac, Hauth⟩⟩
+  -- Specialize Hdwp with the state alloc is stepping into
+  obtain ⟨ℓ₁, Hℓ₁⟩ : ∃ ℓ₁, (ChipMemory.freshSBUFStore sl.memory).fst = .sbufUnboundedIndex ℓ₁ := by
+    simp
+  ispecialize Hdwp ℓ₁
+  rw [Hℓ₁]
+  ispecialize Hdwp Hfrac
+  unfold dwp
+  ispecialize Hdwp { memory := (ChipMemory.freshSBUFStore sl.memory).snd } sr Hauth
+  -- Eliminate the bupd in the dwp
+  -- NB. This is why we duplicated the modality before.
+  refine .trans emp_sep.mp (BIUpdate.mono ?_)
+  -- Obtain the updated resources
+  iintro ⟨p1', p2', HΦ, s1, s2, ⟨n1, n2, %Hstep⟩, H⟩
+  -- Reestablish dwp using the updated resources
+  iexists p1'
+  iexists p2'
+  isplit l [HΦ]
+  · iexact HΦ
+  iexists s1
+  iexists s2
+  isplit r
+  · iexists (n1 + 1)
+    iexists n2
+    ipure_intro
+    obtain ⟨_, _, _, _, SL, _⟩ := Hstep
+    refine ⟨?_, ?_, ?_, ?_, ?_, ?_⟩ <;> try omega
+    refine StepN.step (step.asn <| .sbuf_alloc ?_) SL
+    simp at ⊢ Hℓ₁
+    exact Hℓ₁.symm
+  · iexact H
+
+end weakestpre
+
+/-- Unary weakest preconditions
+
+We can define generic `dwp` proof rules that work whenever one side takes a step independently
+of each other.
+These independent steps are defined semantically, and specified using a `uwpL/uwpR` structures. -/
+structure uwp (DataT : Type _) where
   pre   : PROP DataT
   post  : PROP DataT
-  prog  : ExecState DataT
+  prog  : NML.ExecState DataT
+  prog' : NML.ExecState DataT
   steps : Nat
 
-def UWP.LeftSpec (u : UWP DataT) : PROP DataT :=
-  iprop(∀ σₗ σᵣ, u.pre -∗ state_interp σₗ σᵣ -∗
-    ∀ prog' σₗ', ⌜SmallStep.StepN u.steps (u.prog, σₗ) (prog', σₗ')⌝ -∗ |==> (state_interp σₗ' σᵣ ∗ u.post))
+/-- A `uwp` that uses its resources to take steps on the left. -/
+structure uwpL (DataT : Type _) extends uwp DataT where
+  spec : ⊢ iprop(∀ σₗ σᵣ, pre -∗ state_interp σₗ σᵣ -∗
+    (∃ σₗ', ⌜SmallStep.StepN steps (prog, σₗ) (prog', σₗ')⌝ ∗ |==> (state_interp σₗ' σᵣ ∗ post)))
 
-def UWP.RightSpec (u : UWP DataT) : PROP DataT :=
-  iprop(∀ σₗ σᵣ, u.pre -∗ state_interp σₗ σᵣ -∗
-    ∀ prog' σᵣ', ⌜SmallStep.StepN u.steps (u.prog, σᵣ) (prog', σᵣ')⌝ -∗ |==> (state_interp σₗ σᵣ' ∗ u.post))
+/-- A `uwp` that uses its resources to take steps on the right. -/
+structure uwpR (DataT : Type _) extends uwp DataT where
+  spec : ⊢ iprop(∀ σₗ σᵣ, pre -∗ state_interp σₗ σᵣ -∗
+    (∃ σᵣ', ⌜SmallStep.StepN steps (prog, σᵣ) (prog', σᵣ')⌝ ∗ |==> (state_interp σₗ σᵣ' ∗ post)))
+
+section uwp
+
+open Iris Iris.BI Iris.BI.BIBase KLR.Core Iris NML SmallStep
+
+variable {DataT : Type _}
+
+/-- Step the left-hand side of a dwp using a `uwpL`. -/
+theorem dwpL (u : uwpL DataT) (Hx : u.steps ≤ Lx) :
+    ⊢ (u.post -∗ dwp (Lm - u.steps) Rm (Lx - u.steps) Rx u.prog' pr Φ) -∗
+      u.pre -∗ dwp Lm Rm Lx Rx u.prog pr Φ := by
+  -- Include the spec inside the separating context
+  apply Entails.trans u.spec ?_
+  -- Unfold the dwp in the conclusion
+  conv => rhs; rhs; unfold dwp
+  iintro Hspec Hdwp Hpre sl sr Hs
+  -- Apply the spec to obtain a new post state and an update
+  ispecialize Hspec sl sr Hpre Hs
+  icases Hspec with ⟨sl', %Hstep, Hupd⟩
+  -- Eliminate bupds from the hypotheses but not the conclusion
+  istop
+  refine .trans ?_ bupd_idem.mp
+  refine .trans bupd_frame_l (BIUpdate.mono ?_)
+  iintro ⟨Hdwp, ⟨Hs', Hpost⟩⟩
+  -- Obtain the resources from the dwp, under its bupd
+  ispecialize Hdwp Hpost
+  unfold dwp
+  ispecialize Hdwp sl' sr Hs'
+  refine .trans emp_sep.mp (BIUpdate.mono ?_)
+  iintro ⟨p1', p2', HΦ, sl'', sr'', ⟨n1, n2, %Hstep''⟩, Hs''⟩
+  -- Reestablish the dwp using the new resources
+  iexists p1'
+  iexists p2'
+  isplit l [HΦ]
+  · iexact HΦ
+  iexists sl''
+  iexists sr''
+  isplit r [Hs'']
+  · iexists (n1 + u.steps)
+    iexists n2
+    ipure_intro
+    obtain ⟨_, _, _, _, _, _⟩ := Hstep''
+    refine ⟨?_, ?_, ?_, ?_, ?_, ?_⟩ <;> try omega
+    rw [Nat.add_comm _ _]
+    apply StepN_add_iff.mpr
+    exists (u.prog', sl')
+  · iexact Hs''
+
+/-- Step the right-hand side of a dwp using a `uwpR`. -/
+theorem dwpR (u : uwpR DataT) (Hx : u.steps ≤ Rx) :
+    ⊢ (u.post -∗ dwp Lm (Rm - u.steps) Lx (Rx - u.steps) pl u.prog' Φ) -∗
+      u.pre -∗ dwp Lm Rm Lx Rx pl u.prog Φ := by
+  -- Include the spec inside the separating context
+  apply Entails.trans u.spec ?_
+  -- Unfold the dwp in the conclusion
+  conv => rhs; rhs; unfold dwp
+  iintro Hspec Hdwp Hpre sl sr Hs
+  -- Apply the spec to obtain a new post state and an update
+  ispecialize Hspec sl sr Hpre Hs
+  icases Hspec with ⟨sr', %Hstep, Hupd⟩
+  -- Eliminate bupds from the hypotheses but not the conclusion
+  istop
+  refine .trans ?_ bupd_idem.mp
+  refine .trans bupd_frame_l (BIUpdate.mono ?_)
+  iintro ⟨Hdwp, ⟨Hs', Hpost⟩⟩
+  -- Obtain the resources from the dwp, under its bupd
+  ispecialize Hdwp Hpost
+  unfold dwp
+  ispecialize Hdwp sl sr' Hs'
+  refine .trans emp_sep.mp (BIUpdate.mono ?_)
+  iintro ⟨p1', p2', HΦ, sl'', sr'', ⟨n1, n2, %Hstep''⟩, Hs''⟩
+  -- Reestablish the dwp using the new resources
+  iexists p1'
+  iexists p2'
+  isplit l [HΦ]
+  · iexact HΦ
+  iexists sl''
+  iexists sr''
+  isplit r [Hs'']
+  · iexists n1
+    iexists n2 + u.steps
+    ipure_intro
+    obtain ⟨_, _, _, _, _, _⟩ := Hstep''
+    refine ⟨?_, ?_, ?_, ?_, ?_, ?_⟩ <;> try omega
+    rw [Nat.add_comm _ _]
+    apply StepN_add_iff.mpr
+    exists (u.prog', sr')
+  · iexact Hs''
+
+def uwpPureL {p p' : Prog DataT} (H : PureStep p p') : uwpL DataT where
+  pre   := iprop(True)
+  post  := iprop(True)
+  prog  := p
+  prog' := p'
+  steps := 1
+  spec  := by
+    iintro σₗ σᵣ %_ Hσ
+    iexists σₗ
+    isplit r
+    · ipure_intro
+      exact stepN_1_iff_step.mpr <| H σₗ
+    · refine .trans ?_ BIUpdate.intro
+      refine .trans ?_ sep_true.mpr
+      iintro Hσ
+      iexact Hσ
+
+def uwpPureR {p p' : Prog DataT} (H : PureStep p p') : uwpR DataT where
+  pre   := iprop(True)
+  post  := iprop(True)
+  prog  := p
+  prog' := p'
+  steps := 1
+  spec  := by
+    iintro σₗ σᵣ %_ Hσ
+    iexists σᵣ
+    isplit r
+    · ipure_intro
+      exact stepN_1_iff_step.mpr <| H σᵣ
+    · refine .trans ?_ BIUpdate.intro
+      refine .trans ?_ sep_true.mpr
+      iintro Hσ
+      iexact Hσ
+
+end uwp
+
+
+
+
+
+
+
+
+
+
+/-
 
 def UWP.Frame (u : UWP DataT) (P : PROP DataT) : UWP DataT where
   pre   := iprop(u.pre  ∗ P)
@@ -201,294 +510,4 @@ theorem UWP.rightSpec_frame {u : @UWP DataT} :
   isplit l [HP]
   · iexact HP
   · iexact Hwp
-
-
--- def awp (Lm Rm Lx Rx : Nat) (p1 p2 : ExecState DataT) (Φ : ExecState DataT → ExecState DataT → @PROP DataT) :
---     @PROP DataT :=
---   iprop(∀ sl, ∀ sr, state_interp sl sr -∗
---           ∃ cl', ∃ cr', ∃ nl, ∃ nr,
---           ⌜Lm ≤ nl ∧ Rm ≤ nr ∧ nl ≤ Lx ∧ nr ≤ Rx ∧ SmallStep.StepN nl (p1, sl) cl' ∧ SmallStep.StepN nr (p2, sr) cr'⌝ ∗
---           |==> (state_interp cl'.2 cr'.2 ∗ Φ cl'.1 cr'.1))
-
-def awp (Lm Rm Lx Rx : Nat) (p1 p2 : ExecState DataT) (Φ : ExecState DataT → ExecState DataT → @PROP DataT) :
-    @PROP DataT :=
-  iprop(∀ s1, ∀ s2, state_interp s1 s2 -∗ |==>
-          ∃ p1' p2',
-            Φ p1' p2' ∗
-            ∃ s1' s2',
-              (∃ nl nr, ⌜Lm ≤ nl ∧ Rm ≤ nr ∧ nl ≤ Lx ∧ nr ≤ Rx ∧ SmallStep.StepN nl (p1, s1) (p1', s1') ∧ SmallStep.StepN nr (p2, s2) (p2', s2')⌝ ) ∗
-              state_interp s1' s2')
-
-
-theorem wpDesync {K : LeibnizO Nat} {p1 p2 : ExecState DataT} (Φf : NML.Value DataT → NML.Value DataT → @PROP DataT) :
-    ⊢ awp 1 1 K.1 K.1 p1 p2 (wp K · · Φf) -∗ wp K p1 p2 Φf := by
-  refine Entails.trans ?_ (Q := iprop((awp 1 1 K.car K.car p1 p2 fun x1 x2 => wp K x1 x2 Φf) -∗ ?_)) ?G1
-  case G1 =>
-    apply BI.wand_mono BI.entails_preorder.refl
-    apply (Iris.BI.equiv_iff.mp ?G2).mp
-    case G2=> exact (@wp_unfold DataT K p1 p2 _).symm
-  unfold awp
-  iintro Hawp
-  iright
-  iintro sl sr Hσ
-  ispecialize Hawp sl sr Hσ
-
-  istop
-  apply Iris.BI.BIBase.Entails.trans Iris.BI.emp_sep.mp
-  refine BIUpdate.mono ?_
-  istart
-  iintro ⟨Hawp⟩
-
-
-  icases Hawp with ⟨p1', p2', Hwp, s1', s2', ⟨n1, n2, %Hstep⟩, Hupd⟩
-  simp only []
-  -- Eliminate all bupds
-  iexists (p1', s1')
-  iexists (p2', s2')
-  iexists n1
-  iexists n2
-  isplit r
-  · ipure_intro
-    obtain ⟨_, _, _, _, _, _⟩ := Hstep
-    refine ⟨?_, ?_, ?_, ?_, by trivial⟩ <;> try omega
-  istop
-  refine Entails.trans ?_ Iris.BI.later_intro
-  simp only []
-  istart
-  iintro ⟨Hwp, Hs⟩
-  isplit l [Hs]
-  · iexact Hs
-  · iexact Hwp
-  -- icases Hawp with ⟨cl', cr', nl, nr, %Hstep, H⟩
-  -- iexists cl'
-  -- iexists cr'
-  -- iexists nl
-  -- iexists nr
-  -- isplit r
-  -- · ipure_intro
-  --   obtain ⟨_, _, _, _, _, _⟩ := Hstep
-  --   refine ⟨?_, ?_, ?_, ?_, by trivial⟩ <;> try omega
-  -- -- Eliminate the later and bupd
-  -- istop
-  -- refine Entails.trans ?_ Iris.BI.later_intro
-  -- refine BIUpdate.mono ?_
-  -- simp only []
-  -- istart
-  -- apply BI.entails_wand .rfl
-
-theorem wpResync {m' n' : Nat} {p1 p2 : ExecState DataT} (Φ : ExecState DataT → ExecState DataT → @PROP DataT) :
-    ⊢ Φ p1 p2 -∗ awp 0 0 m' n' p1 p2 Φ := by
-  unfold awp
-  iintro HΦ s1 s2 Hσ
-  istop
-  apply Entails.trans _ BIUpdate.intro
-  istart
-  iintro ⟨HΦ, Hσ⟩
-  iexists p1
-  iexists p2
-  isplit l [HΦ]
-  · iexact HΦ
-  iexists s1
-  iexists s2
-  isplit r
-  · iexists 0
-    iexists 0
-    ipure_intro
-    simp only [Nat.le_refl, Nat.zero_le, true_and]
-    refine ⟨SmallStep.StepN.done rfl, SmallStep.StepN.done rfl⟩
-  iexact Hσ
-
-  -- iexists ⟨p1, s1⟩
-  -- iexists ⟨p2, s2⟩
-  -- iexists 0
-  -- iexists 0
-  -- isplit r
-  -- · ipure_intro
-  --   simp only [Nat.le_refl, Nat.zero_le, true_and]
-  --   refine ⟨SmallStep.StepN.done rfl, SmallStep.StepN.done rfl⟩
-
-  -- -- Eliminate the later and bupd
-  -- istop
-  -- refine Entails.trans ?_ BIUpdate.intro
-  -- simp only []
-  -- istart
-  -- iintro ⟨HΦ, Hσ⟩
-
-  -- isplit l [Hσ]
-  -- · iexact Hσ
-  -- · iexact HΦ
-
-
-theorem awpPureL (Hstep : SmallStep.PureStep p1 p1') (Hx : 0 < Lx := by omega) :
-    ⊢ awp (Lm - 1) Rm (Lx - 1) Rx p1' p2 Φ -∗ awp Lm Rm Lx Rx p1 p2 Φ := by
-  simp at Hx
-  istart
-  unfold awp
-  iintro Hawp
-  iintro sl sr Hσ
-  ispecialize Hawp sl sr Hσ
-  istop
-  apply Iris.BI.BIBase.Entails.trans Iris.BI.emp_sep.mp
-  apply BIUpdate.mono _
-  istart
-  iintro ⟨Hawp⟩
-  icases Hawp with ⟨p1', p2', HΦ, s1', s2', ⟨nl, nr, %Hstep⟩, Hstate⟩
-  iexists p1'
-  iexists p2'
-  isplit l [HΦ]
-  · iexact HΦ
-  iexists s1'
-  iexists s2'
-  isplit r
-  · iexists (nl + 1)
-    iexists nr
-    ipure_intro
-    obtain ⟨_, _, _, _, _, _⟩ := Hstep
-    refine ⟨?_, ?_, ?_, ?_, ?_, ?_⟩ <;> try omega
-    refine SmallStep.StepN.step (Hstep sl) ?_
-    trivial
-  · iexact Hstate
-  -- icases Hawp with ⟨cl', cr', nl, nr, %Hstep', H⟩
-  -- iexists cl'
-  -- iexists cr'
-  -- iexists (nl + 1)
-  -- iexists nr
-  -- isplit r
-  -- · ipure_intro
-  --   obtain ⟨_, _, _, _, _, _⟩ := Hstep'
-  --   refine ⟨?_, ?_, ?_, ?_, ?_, ?_⟩ <;> try omega
-  --   refine SmallStep.StepN.step (Hstep sl) ?_
-  --   trivial
-  -- istop
-  -- refine BIUpdate.mono .rfl
-
-theorem awpPureR (Hstep : SmallStep.PureStep p2 p2') (Hx : 0 < Rx := by omega) :
-    ⊢ awp Lm (Rm - 1) Lx (Rx - 1) p1 p2' Φ -∗ awp Lm Rm Lx Rx p1 p2 Φ := by
-  simp at Hx
-  istart
-  unfold awp
-  iintro Hawp
-  iintro sl sr Hσ
-  ispecialize Hawp sl sr Hσ
-  istop
-  apply Iris.BI.BIBase.Entails.trans Iris.BI.emp_sep.mp
-  apply BIUpdate.mono _
-  istart
-  iintro ⟨Hawp⟩
-  icases Hawp with ⟨p1', p2', HΦ, s1', s2', ⟨nl, nr, %Hstep⟩, H⟩
-  iexists p1'
-  iexists p2'
-  isplit l [HΦ]
-  · iexact HΦ
-  iexists s1'
-  iexists s2'
-  isplit r [H]
-  · iexists nl
-    iexists (nr + 1)
-    ipure_intro
-    obtain ⟨_, _, _, _, _, _⟩ := Hstep
-    refine ⟨?_, ?_, ?_, ?_, ?_, ?_⟩ <;> try omega
-    refine SmallStep.StepN.step (Hstep sr) ?_
-    trivial
-  · iexact H
-  -- icases Hawp with ⟨cl', cr', nl, nr, %Hstep', H⟩
-  -- iexists cl'
-  -- iexists cr'
-  -- iexists nl
-  -- iexists (nr + 1)
-  -- isplit r
-  -- · ipure_intro
-  --   obtain ⟨_, _, _, _, _, _⟩ := Hstep'
-  --   refine ⟨?_, ?_, ?_, ?_, ?_, ?_⟩ <;> try omega
-  --   refine SmallStep.StepN.step (Hstep sr) ?_
-  --   trivial
-  -- istop
-  -- refine BIUpdate.mono .rfl
-
--- -- TODO: Port updates for heaps
--- theorem update_lemma (σₗ σᵣ : NML.State DataT) :
---   state_interp σₗ σᵣ ⊢
---     |==> ∃ ℓₗ ℓᵣ, ℓₗ [S]⇉ₗ∅ ∗ ℓᵣ [S]⇉ᵣ∅ ∗
---     state_interp ⟨(ChipMemory.freshSBUFStore σₗ.1).2⟩ ⟨(ChipMemory.freshSBUFStore σᵣ.1).2⟩ :=
---   sorry
-
-
--- TODO: Unify the left and right pure/stateful desync steps with UWP?
-
-
-theorem update_lemma_left (σₗ σᵣ : NML.State DataT)
-      (HL : ChipMemory.get_store σₗ.memory (.sbufUnboundedIndex ℓ₁) = none):
-  state_interp σₗ σᵣ ⊢ |==> ((ChipMemory.freshSBUFStore σₗ.1).1 ⇉ₗ∅ ∗ state_interp ⟨(ChipMemory.freshSBUFStore σₗ.1).2⟩ σᵣ) :=
-  sorry
-
-theorem awpAllocL (Hx : 0 < Lx := by omega) :
-    ⊢ (∀ ℓₗ, (ℓₗ [S]⇉ₗ∅) -∗
-             awp (Lm - 1) Rm (Lx - 1) Rx (.run <| p1'.map (.bind DataT · x (.uptr <| ChipIndex.sbufUnboundedIndex ℓₗ))) p2 Φ) -∗
-      awp Lm Rm Lx Rx (.run <| ⟨.assign (.some x) (.alloc Memory.sbuf), locₗ⟩ :: p1') p2 Φ := by
-  simp at Hx
-  istart
-  iintro Hawp
-  conv =>
-    rhs
-    unfold awp
-  iintro sl sr Hs
-
-  -- Apply update_lemma
-  istop
-  have X := update_lemma_left sl sr (ℓ₁ := sl.memory.sbufUnbounded.next_fresh) ?G
-  case G =>
-    -- Store get fresh is none
-    simp [ChipMemory.get_store]
-    rw [← AllocHeap.get_fresh (t := sl.memory.sbufUnbounded) (H := sl.memory.sbuf_wf)]
-    rfl
-  have Y := @BI.sep_mono_r (PROP := @PROP DataT) _ _
-              (P := iprop((∀ ℓₗ, (ℓₗ [S]⇉ₗ∅) -∗ awp (Lm - 1) Rm (Lx - 1) Rx (.run <| p1'.map (.bind DataT · x (.uptr <| ChipIndex.sbufUnboundedIndex ℓₗ))) p2 Φ)))
-              _ X
-  apply Entails.trans Y
-  clear X Y
-  simp only []
-  istart
-  iintro ⟨Hawp, Hupd⟩
-
-  istop
-  apply Entails.trans bupd_frame_l
-  apply Entails.trans ?_ bupd_idem.mp
-  apply BIUpdate.mono
-  istart
-  iintro ⟨Hawp, ⟨Hfrac, Hauth⟩⟩
-
-  obtain ⟨ℓ₁, Hℓ₁⟩ : ∃ ℓ₁ : Nat, (ChipMemory.freshSBUFStore sl.memory).fst = .sbufUnboundedIndex ℓ₁ := by
-    simp
-
-  -- Need to be very careful with the unfolding ehre
-  ispecialize Hawp ℓ₁
-  rw [Hℓ₁]
-  ispecialize Hawp Hfrac
-
-  unfold awp
-  ispecialize Hawp { memory := (ChipMemory.freshSBUFStore sl.memory).snd } sr Hauth
-  istop
-  apply Iris.BI.BIBase.Entails.trans Iris.BI.emp_sep.mp
-  apply BIUpdate.mono
-  istart
-  iintro ⟨p1', p2', HΦ, s1, s2, ⟨n1, n2, %Hstep⟩, H⟩
-  iexists p1'
-  iexists p2'
-  isplit l [HΦ]
-  · iexact HΦ
-  iexists s1
-  iexists s2
-  isplit r
-  · iexists (n1 + 1)
-    iexists n2
-    ipure_intro
-    obtain ⟨_, _, _, _, _, _⟩ := Hstep
-    refine ⟨?_, ?_, ?_, ?_, ?_, ?_⟩ <;> try omega
-    rename_i SL  _
-    apply SmallStep.StepN.step _ SL
-    apply NML.step.asn
-    apply ExprStep.sbuf_alloc
-    simp
-    simp at Hℓ₁
-    exact Hℓ₁.symm
-  · iexact H
+-/
